theories/iris_rules.v
@@ -4,7 +4,6 @@ From iris.program_logic Require Import language.
 From iris.proofmode Require Import base tactics classes.
 From iris.base_logic Require Export gen_heap ghost_map proph_map.
 From iris.base_logic.lib Require Export fancy_updates.
-From iris.bi Require Export weakestpre.
 Require Export iris iris_locations iris_properties iris_atomicity stdpp_aux.
 Require Export iris_rules_structural iris_rules_pure iris_rules_control iris_rules_resources iris_rules_calls.
 Require Export datatypes host operations properties opsem.
